$$L_{z}=\sum ^{V}_{v=1}L_{z}^{v}=\sum ^{V}_{v=1}\left\| X^{m}-D^{m}\left( E^{m}\left( X^{m}\right) \right) \right\| _{2}^{2}$$

$$S^{F}=\dfrac{<Q,\widetilde{Q}^{T} >}{\left\| Q\right\| _{2}\left\| \widetilde Q^{T}\right\| _{2}}$$

$$P^{F}=F_{cla}(Q)$$

$$\mathbf{W}_{ij}^{F} =  \begin{cases}  1 & \text{if } i = j, \\ p_{i}^{F} \cdot p_{j}^{F} & \text{if } i \neq j \text{ and } p_{i}^{F} \cdot p_{j}^{F} \geq \tau, \\ 0 & \text{otherwise,} \end{cases}$$

$$\mathcal{L}_{F} = - \mathbf{W}_{ii}^{F} \log \left( \frac{\exp(S_{ii}^{F})}{\sum \exp(S_{ij}^{F})} \right)\sum_{j=1, j \neq i}^{N} -\mathbf{W}_{ij}^{F} \log \left( \frac{\exp(S_{ij}^{F})}{\sum \exp(S_{ij}^{F})} \right).$$

$$\mathcal{L}_{FAC} = \frac{1}{2} \| S^{F} - I \|_{2}^{2}$$

$$P^{k}=F_{cla}(Z^{k})$$

$$\mathbf{W}_{ij}^{kk^{'}} =  \begin{cases}  1 & \text{if } i = j, \\ p_{i}^{k} \cdot p_{j}^{k^{'}} & \text{if } i \neq j \text{ and } p_{i}^{k} \cdot p_{j}^{k^{'}} \geq \tau, \\ 0 & \text{otherwise,} \end{cases}$$

$$S^{kk^{'}}=\dfrac{<Z^{k},(Z^{k^{'}})^{T} >}{\left\| Z^{k}\right\| _{2}\left\| (Z^{k^{'}})^{T}\right\| _{2}}$$

$$\mathcal{L}_{causal} = \sum_{\substack{k, k' \in S \\ k < k'}} \left( -\mathbf{W}_{ii}^{kk^{'}} \log \left( \frac{\exp(S_{ii}^{kk^{'}})}{\sum \exp(S_{ij}^{kk^{'}})} \right)- \sum_{j=1, j \neq i}^{N} \mathbf{W}_{ij}^{kk^{'}} \log \left( \frac{\exp(S_{ij}^{kk^{'}})}{\sum \exp(S_{ij}^{kk^{'}})} \right) \right),$$

$$\mathcal{L}_{align} = \frac{1}{\binom{2}{\lvert S \rvert}} \sum_{\substack{k, k' \in S \\ k < k'}} \| \mathbf{W}^{F} - \mathbf{W}^{kk^{'}} \|_{2}^{2},$$

$$\mathcal{L} = \mathcal{L}_{z} + \alpha \mathcal{L}_{F} + \beta \mathcal{L}_{causal} + \mu \mathcal{L}_{align},$$

$$U=\sum ^{V}_{v=1}\dfrac{e^{w^{v}_{\alpha}}}{\sum ^{V}_{k=1}e^{w^{k}_{\alpha}}}H^{v }$$

$$\beta(H^{v}) = \mu(H^{v}) + \epsilon_\mu \Sigma_\mu(H^{v}), \quad \epsilon_\mu \sim \mathcal{N}(0, 1),$$

$$\gamma(H^{v}) = \sigma(H^{v}) + \epsilon_\sigma \Sigma_\sigma(H^{v}), \quad \epsilon_\sigma \sim \mathcal{N}(0, 1),$$â€‹

$$\widetilde H^{v} = \gamma(H^{v}) \left( \frac{H^{v} - \mu(H^{v})}{\sigma(H^{v})} \right) + \beta(H^{v}).$$

